# baseURI: http://topbraid.org/sparqlmotion
# imports: http://spinrdf.org/spl

# c14n-version: 3
@prefix daml: <http://www.daml.org/2001/03/daml+oil#> .
@prefix owl: <http://www.w3.org/2002/07/owl#> .
@prefix rdf: <http://www.w3.org/1999/02/22-rdf-syntax-ns#> .
@prefix rdfs: <http://www.w3.org/2000/01/rdf-schema#> .
@prefix sm: <http://topbraid.org/sparqlmotion#> .
@prefix sml: <http://topbraid.org/sparqlmotionlib#> .
@prefix sp: <http://spinrdf.org/sp#> .
@prefix spin: <http://spinrdf.org/spin#> .
@prefix spl: <http://spinrdf.org/spl#> .
@prefix xsd: <http://www.w3.org/2001/XMLSchema#> .
sp:_defaultValue
  rdf:type sp:Variable ;
  sp:varName "defaultValue"^^xsd:string ;
.
sp:_predicate
  rdf:type sp:Variable ;
  sp:varName "predicate"^^xsd:string ;
.
sp:_restriction
  rdf:type sp:Variable ;
  sp:varName "restriction"^^xsd:string ;
.
sp:_type
  rdf:type sp:Variable ;
  sp:varName "type"^^xsd:string ;
.
spin:Functions
  spin:constraint [
      rdf:type spl:Attribute ;
      spl:defaultValue "result"^^xsd:string ;
      spl:maxCount 1 ;
      spl:minCount 0 ;
      spl:predicate sm:outputVariable ;
      spl:valueType xsd:string ;
      rdfs:comment "The name of the result variable. In SPARQLMotion, a result variable must be specified, but we leave the minCount constraint on 0 to remove clutter in constraint checking."^^xsd:string ;
    ] ;
.
<http://topbraid.org/sparqlmotion>
  rdf:type owl:Ontology ;
  rdfs:comment "Core ontology of SPARQLMotion: a declarative scripting language for Semantic Web technology. This ontology defines the basic building blocks of SPARQLMotion scripts. Scripts consist of modules, which are instances of (some subclass of) sm:Module. Modules can be chained together using sm:next and the sm:child properties." ;
  rdfs:seeAlso <http://sparqlmotion.org> ;
  owl:imports <http://spinrdf.org/spl> ;
  owl:versionInfo "2.3"^^xsd:string ;
.
sm:CSV
  rdf:type sm:ValueType ;
  rdfs:label "CSV"^^xsd:string ;
.
sm:Function
  rdf:type rdfs:Class ;
  rdfs:comment """A SPIN Function backed by a SPARQLMotion script. When the function is called, the body script will be executed. Can also be called as web service using a SM servlet container such as the TopBraid Live.

There are two ways of defining the body script:
- sm:bodyScript for linear scripts (and XML Syntax)
- sm:returnModule for any other style (and graphical notation)"""^^xsd:string ;
  rdfs:label "Function"^^xsd:string ;
  rdfs:subClassOf spin:Function ;
.
sm:Functions
  rdf:type sm:Function ;
  spin:abstract "true"^^xsd:boolean ;
  rdfs:comment "An abstract superclass grouping together SPARQLMotion Functions."^^xsd:string ;
  rdfs:label "Functions"^^xsd:string ;
  rdfs:subClassOf spin:Functions ;
.
sm:JSON
  rdf:type sm:ValueType ;
  rdfs:label "JSON"^^xsd:string ;
.
sm:Module
  rdf:type rdfs:Class ;
  rdfs:comment """The metaclass of SPARQLMotion modules. SPARQLMotion modules are SPIN Modules that can perform some arbitrary data processing task.
The instances of this metaclass define the input properties that are used to control the behavior. In order to declare a property, the following two SPIN templates must be used (attached to the class via spin:constraint):
- spl:Argument: this is the most common case for single-valued properties that are configured by the user. In addition to concrete RDF nodes, spl:Arguments can also point to a SPARQL SELECT query (sp:Select), a SPIN Template call, or a SPARQL expression. In those cases, the value of the property will be computed dynamically at execution time. The nested SPARQL expressions can access any pre-bound input variable.
- spl:Attribute: this should be used for any other value, such as SPARQL queries that drive the behavior of the module. No inline queries are supported for spl:Attributes."""^^xsd:string ;
  rdfs:label "Module"^^xsd:string ;
  rdfs:subClassOf spin:Module ;
.
sm:Modules
  rdf:type rdfs:Class ;
  spin:abstract "true"^^xsd:boolean ;
  spin:constructor [
      rdf:type spl:ConstructDefaultValues ;
    ] ;
  rdfs:comment "The abstract base class for the various types of SPARQLMotion data processing modules." ;
  rdfs:label "Modules"^^xsd:string ;
  rdfs:subClassOf spin:Modules ;
.
sm:SelectTemplates
  rdf:type spin:SelectTemplate ;
  spin:abstract "true"^^xsd:boolean ;
  spin:constraint [
      rdf:type spl:Attribute ;
      spl:maxCount 1 ;
      spl:minCount 1 ;
      spl:predicate sm:body ;
      rdfs:comment "The body script of the template. Will be executed for each row of the result set."^^xsd:string ;
    ] ;
  rdfs:comment "Root class of SPARQLMotion modules that are based on SPIN templates. Subclasses of this should also have rdf:type sm:Module. The SPARQLMotion engine will execute the SELECT query specified as spin:body of the module and repeat the sm:body of the module in each iteration, with pre-bound variables for each binding in the result set row."^^xsd:string ;
  rdfs:label "Select templates"^^xsd:string ;
  rdfs:subClassOf spin:SelectTemplates ;
.
sm:TSV
  rdf:type sm:ValueType ;
  rdfs:label "TSV"^^xsd:string ;
.
sm:ValueType
  rdf:type rdfs:Class ;
  rdfs:comment "A value type such as XML or JSON." ;
  rdfs:label "value type" ;
  rdfs:subClassOf rdfs:Resource ;
.
sm:XML
  rdf:type sm:ValueType ;
  rdfs:label "XML"^^xsd:string ;
.
sm:body
  rdf:type rdf:Property ;
  rdfs:comment "Links an iterator modules with its body, i.e. the start of a module chain that is executed as part of the loop." ;
  rdfs:label "body"^^xsd:string ;
  rdfs:range spin:Modules ;
  rdfs:subPropertyOf sm:child ;
.
sm:bodyScript
  rdf:type rdf:Property ;
  rdf:type owl:DeprecatedProperty ;
  rdfs:comment """Links a SPARQLMotion Function with the beginning of the linear SM script that shall be executed when the function is called.

This mechanism has been deprecated as of TopBraid 3.6.2. The preferred mechanism is to embed SM modules into the XML syntax of SWP."""^^xsd:string ;
  rdfs:domain sm:Function ;
  rdfs:label "body script"^^xsd:string ;
  rdfs:range sm:Modules ;
.
sm:child
  rdf:type rdf:Property ;
  rdfs:comment "Links a parent module with a child module that marks the start of a nested sub-script. This property is not meant to be used directly, but its primary function is to serve as superproperty of sm:body, sm:if and sm:else." ;
  rdfs:label "child"^^xsd:string ;
  rdfs:range spin:Modules ;
.
sm:else
  rdf:type rdf:Property ;
  rdfs:comment "Links a branching module with its \"false\" branch, i.e. the branch that shall be executed if the condition is false." ;
  rdfs:label "else"^^xsd:string ;
  rdfs:range spin:Modules ;
  rdfs:subPropertyOf sm:child ;
.
sm:icon
  rdf:type rdf:Property ;
  rdfs:comment "Can link a sm:Module subclass with an image URL so that the module can be displayed in visual editors. Images should be 48x48 pixels and in PNG, GIF or JPG format." ;
  rdfs:label "icon"^^xsd:string ;
.
sm:if
  rdf:type rdf:Property ;
  rdfs:comment "Links a branching module with its \"true\" branch, i.e. the branch that shall be executed if the condition is true." ;
  rdfs:label "if"^^xsd:string ;
  rdfs:range spin:Modules ;
  rdfs:subPropertyOf sm:child ;
.
sm:next
  rdf:type rdf:Property ;
  rdfs:comment "Links a source module (subject) with a target module (object), describing a chain of execution and evaluation." ;
  rdfs:domain spin:Modules ;
  rdfs:label "next"^^xsd:string ;
  rdfs:range spin:Modules ;
.
sm:nodeX
  rdf:type rdf:Property ;
  rdfs:comment "The x coordinate of a module on a diagram." ;
  rdfs:label "node x"^^xsd:string ;
  rdfs:range xsd:integer ;
.
sm:nodeY
  rdf:type rdf:Property ;
  rdfs:comment "The y coordinate of a module on a diagram." ;
  rdfs:label "node y"^^xsd:string ;
  rdfs:range xsd:integer ;
.
sm:outputVariable
  rdf:type rdf:Property ;
  rdfs:comment "The name of the declared output variable of a module. This is typically used by modules to enable script users to bind the output of a module with matching variables in the target module." ;
  rdfs:label "outputVariable" ;
  rdfs:range xsd:string ;
.
sm:returnModule
  rdf:type rdf:Property ;
  rdfs:comment "Can be attached to user-defined SPARQLMotion functions to define the return module of the function's SPARQLMotion script. The result of the function will depend on the selected return module type."^^xsd:string ;
  rdfs:domain spin:Function ;
  rdfs:label "return module"^^xsd:string ;
  rdfs:range sm:Modules ;
.
sm:source
  rdf:type owl:AnnotationProperty ;
  rdfs:comment "Can be used to link a resource to the SPARQLMotion script that generated it. For example, if a file has been automatically generated by a SPARQLMotion script then the owl:Ontology in the resulting file should point back to the script, so that others can re-run the generation if the input data has changed." ;
  rdfs:label "source"^^xsd:string ;
  rdfs:subPropertyOf rdfs:seeAlso ;
.
